**Primera seccion**

**1.1**

A =             B =           A+B =
    |2 3|           |1 5|           |3 8|
    |4 1|           |0 2|           |4 3|


**1.2**
A =                 B =                 A+B =
    |1 2 3|             |9 8 7|               |10 10 10|
    |4 5 6|             |6 5 4|               |10 10 10|
    |7 8 9|             |3 2 1|               |10 10 10|


**1.3**
Demuestre que (A + B) + C = A + (B + C)

A =             B =             C =             A+B =               (A + B) + C =
    | 1 0 |         | 4 -1|         | 3 2 |           | 5 -1 |                    | 8 1 |
    |-2 3 |         | 2 0 |         |-1 1 |           | 0  3 |                    |-1 4 |


A =             B =             C =             B+C =               A + (B + C) =
    | 1 0 |         | 4 -1|         | 3 2 |           | 7 1 |                     | 8 1 |
    |-2 3 |         | 2 0 |         |-1 1 |           | 1 1 |                     |-1 4 |

**1.4**

A =             B =                 A+B =
    |2 3|           | 5 6 7 |               esta operacion no es posible ya que las matrices son de dimensiones diferentes
    |4 1|           | 8 9 10|               
